Prove a (weak) recovery interpretation proof
Currently makes assumptions that are too strong about how the recovery
procedure works (everything requires the invariant and that the
abstraction is preserved, which isn't even true for the replicated
disk). Nonetheless the structure is present even with this proof, and
there are TODOs marking where I think crash invariant handling should be
added.

src/Shallow/Interpret.v
@@ -30,6 +30,8 @@ Section Interpreter.
 
   Notation exec1 := (exec step1).
   Notation exec2 := (exec step2).
+  Notation rexec1 := (rexec step1).
+  Notation rexec2 := (rexec step2).
 
   (* TODO: in general, it might not be the case that crash states line up with
   abstract states as desired; there might be states that are only exposed by
@@ -48,14 +50,16 @@ Section Interpreter.
     | Crashed state => invariant state
     end.
 
-  Hint Constructors exec.
-
+  (* TODO: this property shouldn't be called interpretation, need a more
+  intuitive name *)
   Definition interpretation :=
     forall T (p: prog2 T) state r,
       invariant state ->
       exec1 (interpret p) state r ->
       exec2 p (abstraction state) (res_abstraction r) /\
       res_invariant r.
+
+  Hint Constructors exec.
 
   Theorem interpret_exec :
     (* every operation is implemented according to the step semantics of the
@@ -106,6 +110,34 @@ Section Interpreter.
         intuition eauto.
   Qed.
 
+  Definition rres_abstraction T R (r: RResult State1 T R) : RResult State2 T R :=
+    match r with
+    | RFinished v state => RFinished v (abstraction state)
+    | Recovered v state => Recovered v (abstraction state)
+    end.
+
+  Definition rres_invariant T R (r: RResult State1 T R) : Prop :=
+    match r with
+    | RFinished _ state => invariant state
+    | Recovered _ state => invariant state
+    end.
+
+  Variable rec: prog1 unit.
+
+  Definition exec_recover_interpretation :=
+    forall R (pr: prog2 R) state rv state',
+      invariant state ->
+      exec_recover step1 (Bind rec (fun _ => interpret pr)) state rv state' ->
+      exec_recover step2 pr (abstraction state) rv (abstraction state') /\
+      invariant state'.
+
+  Definition rexec_interpretation :=
+    forall T (p: prog2 T) R (pr: prog2 R) state r,
+      invariant state ->
+      rexec1 (interpret p) (Bind rec (fun _ => interpret pr)) state r ->
+      rexec2 p pr (abstraction state) (rres_abstraction r) /\
+      rres_invariant r.
+
 End Interpreter.
 
 Theorem interpretation_weaken : forall `(step1: Semantics opT1 State1)
@@ -124,3 +156,100 @@ Proof.
   eapply H0; eauto.
   eapply H0; eauto.
 Qed.
+
+Section InterpretRexec.
+
+  Context `(step1: Semantics opT1 State1) `(step2: Semantics opT2 State2)
+          (op_impl: forall T, opT2 T -> prog opT1 T)
+          (invariant: State1 -> Prop)
+          (abstraction: State1 -> State2).
+
+  (* for now, recovery must make all changes to state and cannot preserve
+     its return value
+
+     TODO: for log, need to generalize this or have recovery store result in
+     variable *)
+  Variable (rec: prog opT1 unit).
+
+  Hypothesis
+    (Hinterp:
+       interpretation op_impl step1 step2 invariant abstraction).
+
+  Hypothesis
+      (Hrec: forall state r, exec step1 rec state r ->
+                    (* TODO: should be crash invariant *)
+                    invariant state ->
+                    (* TODO: should mix invariant for Finished and crash
+                    invariant for Crashed *)
+                    res_invariant invariant r /\
+                    match r with
+                    | Finished _ state' =>
+                      (* TODO: too strong - what the recovery procedure needs to
+                         guarantee is that it preserves the crash abstractions
+                         of [interpret p] (that is, when [state] is a crash state of
+                         [interpret p], the recovery can produce [state'] with an
+                         abstraction)
+
+                         Note that this can be phrased as a per-operation
+                         assumption that implies a property about all
+                         interpreted programs. *)
+                      abstraction state' = abstraction state
+                    | Crashed state' =>
+                      (* TODO: in this case, similar to Finished case we will
+                      guarantee the abstraction is from some crash state, but
+                      will not guarantee the invariant in res_invariant but only
+                      the crash invariant (sufficient for idempotency) *)
+                      abstraction state' = abstraction state
+                    end).
+
+  Set Default Proof Using "All".
+
+  Ltac cleanup := simpl in *; eauto; safe_intuition;
+                  try match goal with
+                      | |- _ /\ _ =>
+                        split; [ | solve [ eauto ]]
+                      end.
+
+  Hint Constructors exec_recover.
+
+  Ltac forward_specs :=
+    repeat match goal with
+           | [ H: exec _ rec _ _ |- _ ] =>
+             eapply Hrec in H; cleanup
+           | [ H: exec _ (interpret _ _) _ _ |- _ ] =>
+             eapply Hinterp in H; cleanup
+           end;
+    repeat match goal with
+             (* TODO: this will have to be more sophisticated with proper
+             recovery crash correctness handling *)
+           | [ H: abstraction _ = abstraction _ |- _ ] =>
+             rewrite H in *
+           end;
+    eauto.
+
+  Theorem interpret_exec_recover :
+      exec_recover_interpretation op_impl step1 step2 invariant abstraction rec.
+  Proof.
+    unfold interpretation, exec_recover_interpretation; intros.
+    induction H0.
+    - inv_exec; forward_specs.
+    - inv_exec; forward_specs.
+  Qed.
+
+  Hint Constructors rexec.
+
+  Theorem interpret_rexec :
+      rexec_interpretation op_impl step1 step2 invariant abstraction rec.
+  Proof.
+    unfold interpretation, rexec_interpretation; intros.
+    match goal with
+    | [ H: rexec _ _ _ _ _ |- _ ] =>
+      inversion H; subst; repeat sigT_eq
+    end.
+    - simpl; forward_specs.
+    - simpl; forward_specs.
+      eapply interpret_exec_recover in H2; cleanup.
+      eauto.
+  Qed.
+
+End InterpretRexec.
